Validate submission 8318f2d8-c6c2-4d95-9d15-8629720a06d7
Co-authored-by: hybridnoise <9207260+hybridnoise@users.noreply.github.com>

Challenge/Ripemd160/Submission/Proofs/Bytecode/JointRightPackRaw.lean
@@ -31,11 +31,11 @@ structure Input where
   limit : UInt256
 def template : List Instr :=
   [ .op (.Swap ⟨3, by decide⟩),
-    .op (.Dup ⟨3, by decide⟩),
-    .op (.Dup ⟨5, by decide⟩),
+    .op (.Dup ⟨2, by decide⟩),
+    .op (.Dup ⟨4, by decide⟩),
+    .op (.Dup ⟨6, by decide⟩),
     .op .NOT,
     .op .OR,
-    .op (.Dup ⟨3, by decide⟩),
     .op .XOR,
     .op .ADD,
     .push ⟨1, by decide⟩ (UInt256.ofNat 252),
@@ -92,7 +92,7 @@ def actualOutput (memory : ByteArray) (x : Input) (rho : List UInt256) : List UI
   [ (UInt256.lor (UInt256.shiftLeft x.lower (UInt256.ofNat 144)) x.lower),
     (UInt256.shiftLeft x.lower (UInt256.ofNat 144)),
     (UInt256.lor x.h4 (UInt256.shiftLeft x.rd (UInt256.ofNat 144))),
-    (UInt256.lor x.h1 (UInt256.shiftLeft (UInt256.land x.lower (UInt256.add x.re (UInt256.shiftRight (UInt256.mul x.factor (UInt256.land x.lower (UInt256.add (UInt256.add (MachineState.readWord memory 252) (UInt256.add (UInt256.xor x.rb (UInt256.lor (UInt256.lnot x.rd) x.rc)) x.ra)) x.k))) (UInt256.ofNat 29)))) (UInt256.ofNat 144))),
+    (UInt256.lor x.h1 (UInt256.shiftLeft (UInt256.land x.lower (UInt256.add x.re (UInt256.shiftRight (UInt256.mul x.factor (UInt256.land x.lower (UInt256.add (UInt256.add (MachineState.readWord memory 252) (UInt256.add (UInt256.xor (UInt256.lor (UInt256.lnot x.rd) x.rc) x.rb) x.ra)) x.k))) (UInt256.ofNat 29)))) (UInt256.ofNat 144))),
     (UInt256.lor x.h0 (UInt256.shiftLeft x.re (UInt256.ofNat 144))),
     (UInt256.lor x.h3 (UInt256.shiftLeft (UInt256.shiftRight (UInt256.mul x.factor x.rc) (UInt256.ofNat 28)) (UInt256.ofNat 144))),
     (UInt256.lor x.h2 (UInt256.shiftLeft x.rb (UInt256.ofNat 144))),
